rpc: Used saved_preds, most of MakeRPCClient

src/program_proof/memkv/rpc_proof.v
@@ -1,14 +1,23 @@
 From Goose.github_com.mit_pdos.gokv.urpc Require Import rpc.
+From iris.base_logic.lib Require Import saved_prop.
 From Perennial.program_proof Require Import dist_prelude.
 From Perennial.program_proof Require Import marshal_proof.
 From Perennial.algebra Require Import auth_map.
 From Perennial.base_logic Require Export lib.ghost_map lib.mono_nat.
 
+Record rpc_reg_entry := RegEntry {
+  rpc_reg_rpcid  : u64;
+  rpc_reg_auxtype : Type;
+  rpc_reg_aux : rpc_reg_auxtype;
+  rpc_reg_args : list u8;
+  rpc_reg_saved : gname;
+}.
+
 Class rpcregG (Σ : gFunctors) := RpcRegG {
   rpcreg_mono_natG :> mono_natG Σ;
-  (* mapping from seqno to rpcid and x argument of Pre/Post, and arguments of rpc  *)
-  rpcreg_mapG :> mapG Σ u64 (u64 * { X : Type & X } * list u8);
+  rpcreg_mapG :> mapG Σ u64 rpc_reg_entry;
   rpcreg_escrowG :> mapG Σ u64 unit;
+  rpcreg_savedG :> savedPredG Σ (list u8);
 }.
 
 Section rpc_proof.
@@ -27,35 +36,34 @@ Definition urpc_clientN : namespace := nroot.@"urpc_client".
 Definition urpc_lockN : namespace := nroot.@"urpc_lock".
 
 Record client_chan_gnames := {
-  ccmnat_name : gname;
   ccmapping_name : gname;
   ccescrow_name : gname;
   ccextracted_name : gname;
 }.
 
-Definition client_chan_inner (Γ : client_chan_gnames) (host: u64) (specs : rpc_spec_map) : iProp Σ :=
+Definition client_chan_inner (Γ : client_chan_gnames) (host: u64) : iProp Σ :=
   ∃ ms, "Hchan" ∷ host c↦ ms ∗
   "Hmessages" ∷ [∗ set] m ∈ ms,
-    ∃ (rpcid seqno : u64) reqData replyData X Pre Post (x : X),
+    ∃ (rpcid seqno : u64) reqData replyData X Post (x : X) γ,
        "%Henc" ∷ ⌜ has_encoding (msg_data m) [EncUInt64 seqno;
                                               EncUInt64 (length replyData); EncBytes replyData] ⌝ ∗
-       "%Hlookup_spec" ∷ ⌜ specs !! rpcid = Some (existT X (Pre, Post)) ⌝ ∗
-       "#Hseqno" ∷ ptsto_ro (ccmapping_name Γ) seqno (rpcid, existT X x, reqData) ∗
+       "#Hseqno" ∷ ptsto_ro (ccmapping_name Γ) seqno (RegEntry rpcid X x reqData γ) ∗
+       "HPost_saved" ∷ saved_pred_own γ (Post x reqData) ∗
        "HPost" ∷ (Post x reqData replyData ∨ ptsto_mut (ccescrow_name Γ) seqno 1 tt)
 .
 
 Definition server_chan_inner (host: u64) (specs : rpc_spec_map) : iProp Σ :=
   ∃ ms, "Hchan" ∷ host c↦ ms ∗
   "Hmessages" ∷ [∗ set] m ∈ ms,
-    ∃ rpcid seqno args X Pre Post (x : X) Γ,
+    ∃ rpcid seqno args X Pre Post (x : X) Γ γ,
        "%Henc" ∷ ⌜ has_encoding (msg_data m) [EncUInt64 rpcid; EncUInt64 seqno;
                                               EncUInt64 (length args); EncBytes args] ⌝ ∗
        "%Hlookup_spec" ∷ ⌜ specs !! rpcid = Some (existT X (Pre, Post)) ⌝ ∗
-       "#Hseqno" ∷ ptsto_ro (ccmapping_name Γ) seqno (rpcid, existT X x, args) ∗
+       "#Hseqno" ∷ ptsto_ro (ccmapping_name Γ) seqno (RegEntry rpcid X x args γ) ∗
        "HPre" ∷ □ (Pre x args) ∗
-       "Hclient_chan_inv" ∷ inv urpc_clientN (client_chan_inner Γ (msg_sender m) specs)
+       "HPost_saved" ∷ saved_pred_own γ (Post x args) ∗
+       "Hclient_chan_inv" ∷ inv urpc_clientN (client_chan_inner Γ (msg_sender m))
 .
-
 
 Definition handler_is : ∀ (X:Type) (host:u64) (rpcid:u64) (Pre:X → list u8 → iProp Σ)
                           (Post:X → list u8 → list u8 → iProp Σ), iProp Σ :=
@@ -67,15 +75,9 @@ Definition handler_is : ∀ (X:Type) (host:u64) (rpcid:u64) (Pre:X → list u8 �
 Global Instance handler_is_pers_instance X host rpcid pre post : Persistent (handler_is X host rpcid pre post).
 Proof. apply _. Qed.
 
-(* TODO: either need to revert back to having a fixed global map of (host id, rpcid -> pre/post),
-   or this needs to use saved preds to have the linkage between the RPC Pre/Post and what's stored here.
-
-   The tricky bit here is that the axiomatized spec would require that RPCClient_lock_inner be initialized
-   without even knowing what the rpc_spec_map is: the precondition is just true, only actual calls have
-   handler_is assumptions *)
 Definition RPCClient_lock_inner Γ (cl : loc) (host : u64) mref : iProp Σ :=
   ∃ pending reqs estoks extoks (n : u64),
-            "%Hdom_range" ∷ ⌜ ∀ id, (int.Z id ≤ int.Z n)%Z ↔ id ∈ dom (gset u64) reqs ⌝ ∗
+            "%Hdom_range" ∷ ⌜ ∀ id, (0 < int.Z id < int.Z n)%Z ↔ id ∈ dom (gset u64) reqs ⌝ ∗
             "%Hdom_eq" ∷ ⌜ dom (gset u64) reqs = dom (gset u64) estoks ∧
                                     dom (gset u64) reqs = dom (gset u64) extoks ⌝ ∗
             "%Hdom_pending" ∷ ⌜ dom (gset u64) pending ⊆ dom (gset u64) reqs  ⌝ ∗
@@ -84,27 +86,39 @@ Definition RPCClient_lock_inner Γ (cl : loc) (host : u64) mref : iProp Σ :=
             "Hescrow_ctx" ∷ map_ctx (ccescrow_name Γ) 1 estoks ∗
             "Hescrow_ctx" ∷ map_ctx (ccextracted_name Γ) 1 extoks ∗
             "Hpending_map" ∷ map.is_map mref (pending, zero_val (struct.ptrT callback)) ∗
-            "Hreqs" ∷ [∗ map] seqno ↦ req ∈ reqs, ptsto_ro (ccmapping_name Γ) seqno req ∗
-                 let rpcid := fst req in
-          (*       let X := projT1 (snd req) in
-                 let x : X := projT2 (snd req) in *)
-                 (* Each request is in one of 3 states: *)
+            "Hreqs" ∷ [∗ map] seqno ↦ req ∈ reqs, ∃ (Post : rpc_reg_auxtype req → list u8 → list u8 → iProp Σ),
+                 "Hreg_entry" ∷  ptsto_ro (ccmapping_name Γ) seqno req ∗
+                 "HPost_saved" ∷ saved_pred_own (rpc_reg_saved req) (Post (rpc_reg_aux req) (rpc_reg_args req)) ∗
                  (* (1) Reply thread has not yet processed, so it is in pending
                     and we have escrow token *)
                  (∃ cb, ⌜ pending !! seqno  = Some cb ⌝ ∗ ptsto_mut (ccescrow_name Γ) seqno 1 tt ∗
                           (* TODO: cb ownership *) True) ∨
                  (* (2) Reply thread has received message, removed from pending,
                     but caller has not extracted ownership *)
-                 (∃ cb : unit, ⌜ pending !! seqno  = None ⌝ ∗ (* TODO: cb ownership *) True ) ∨
+                 (∃ reply (cb : unit), ⌜ pending !! seqno  = None ⌝ ∗ (* TODO: cb ownership *) True ∗
+                               (Post (rpc_reg_aux req) (rpc_reg_args req) reply)) ∨
                  (* (3) Caller has extracted ownership *)
                  (⌜ pending !! seqno  = None ⌝ ∗ ptsto_mut (ccextracted_name Γ) seqno 1 tt).
 
 Definition RPCClient_own (cl : loc) (host:u64) : iProp Σ :=
   ∃ Γ lk r (mref : loc),
-    "Hstfields" ∷ ("mu" ∷ readonly (cl ↦[RPCClient :: "mu"] #lk) ∗
-    "send" ∷ readonly (cl ↦[RPCClient :: "send"] send_endpoint host r) ∗
-    "pending" ∷ readonly (cl ↦[RPCClient :: "pending"] #mref)) ∗
-    "Hlk" ∷ is_lock urpc_lockN #lk (RPCClient_lock_inner Γ cl host mref).
+    "#Hstfields" ∷ ("mu" ∷ readonly (cl ↦[RPCClient :: "mu"] #lk) ∗
+    "#send" ∷ readonly (cl ↦[RPCClient :: "send"] send_endpoint host r) ∗
+    "#pending" ∷ readonly (cl ↦[RPCClient :: "pending"] #mref)) ∗
+    "#Hchan" ∷ inv urpc_clientN (client_chan_inner Γ r) ∗
+    "#Hlk" ∷ is_lock urpc_lockN #lk (RPCClient_lock_inner Γ cl host mref).
+
+Definition RPCClient_reply_own (cl : loc) (r : chan) : iProp Σ :=
+  ∃ Γ host lk (mref : loc),
+    "#Hstfields" ∷ ("mu" ∷ readonly (cl ↦[RPCClient :: "mu"] #lk) ∗
+    "#pending" ∷ readonly (cl ↦[RPCClient :: "pending"] #mref)) ∗
+    "#Hchan" ∷ inv urpc_clientN (client_chan_inner Γ r) ∗
+    "#Hlk" ∷ is_lock urpc_lockN #lk (RPCClient_lock_inner Γ cl host mref).
+
+Lemma wp_RPCClient__replyThread cl r :
+  RPCClient_reply_own cl r -∗
+  WP RPCClient__replyThread #cl (recv_endpoint r) {{ _, True }}.
+Proof. Admitted.
 
 Lemma wp_MakeRPCClient (host:u64):
   {{{
@@ -139,6 +153,33 @@ Proof.
   iNamed "Hcl".
   iDestruct (struct_fields_split with "Hcl") as "Hcl". iNamed "Hcl".
   wp_pures.
-Abort.
+  (* TODO: why do I have to unshelve this, when in other cases it appears to get picked up automatically *)
+  unshelve (iMod (readonly_alloc_1 with "mu") as "#mu"); [| apply _ |].
+  unshelve (iMod (readonly_alloc_1 with "send") as "#send"); [| apply _ |].
+  unshelve (iMod (readonly_alloc_1 with "pending") as "#pending"); [| apply _ |].
+
+  iMod (map_init (∅ : gmap u64 rpc_reg_entry)) as (γccmapping) "Hmapping_ctx".
+  iMod (map_init (∅ : gmap u64 unit)) as (γccescrow) "Hescrow_ctx".
+  iMod (map_init (∅ : gmap u64 unit)) as (γccextracted) "Hextracted_ctx".
+  set (Γ := {| ccmapping_name := γccmapping; ccescrow_name := γccescrow;
+               ccextracted_name := γccextracted |}).
+  iMod (alloc_lock urpc_lockN _ _ (RPCClient_lock_inner Γ cl host mref) with
+            "Hfree [Hmapping_ctx Hescrow_ctx Hextracted_ctx seq Hmref]") as "#Hlock".
+  { iNext. iExists ∅, ∅, ∅, ∅, _. iFrame.
+    rewrite ?dom_empty_L.
+    iSplit.
+    { iPureIntro. split; last by set_solver. word. }
+    iSplit; first done.
+    iSplit; first done.
+    rewrite big_sepM_empty //.
+  }
+  iMod (inv_alloc urpc_clientN _ (client_chan_inner Γ r) with "[Hr]") as "#Hchan_inv".
+  { iNext. iExists ∅. iFrame. rewrite big_sepS_empty //. }
+  wp_bind (Fork _).
+  iApply wp_fork.
+  { iNext. wp_pures. iApply wp_RPCClient__replyThread. iExists _, _, _, _. iFrame "#". }
+  iNext. wp_pures. iModIntro. iApply "HΦ".
+  iExists _, _, _, _. iFrame "#".
+Admitted.
 
 End rpc_proof.
